template-rocq/theories/Ast.v
@@ -341,6 +341,22 @@ Proof.
   intros [] []; unfold map_branch; cbn. f_equal. now apply H0.
 Qed.
 
+Lemma tfix_gen_forallb_map_spec {A B} {P : aname -> Prop} {P' P'' : A -> Prop} {p p' p''} {l}
+  {f f' : aname -> aname} {g g' h h' : A -> B} :
+  tFixProp_gen P P' P'' l ->
+  forallb (test_def_gen p p' p'') l ->
+  (forall x, P x -> p x -> f x = f' x) ->
+  (forall x, P' x -> p' x -> g x = g' x) ->
+  (forall x, P'' x -> p'' x -> h x = h' x) ->
+  map (map_def_gen f g h) l = map (map_def_gen f' g' h') l.
+Proof.
+  intros. eapply All_map_eq; red in X. apply forallb_All in H.
+  eapply All_impl.
+  - eapply All_prod. exact X. exact H.
+  - intros [] [[[]] ?]; unfold map_def_gen, test_def_gen in *; cbn in *.
+    rtoProp. f_equal; eauto.
+Qed.
+
 Lemma tfix_forallb_map_spec {A B} {P P' : A -> Prop} {p p'} {l} {f f' g g' : A -> B} :
   tFixProp P P' l ->
   forallb (test_def p p') l ->
@@ -348,11 +364,7 @@ Lemma tfix_forallb_map_spec {A B} {P P' : A -> Prop} {p p'} {l} {f f' g g' : A -
   (forall x, P' x -> p' x -> f' x = g' x) ->
   map (map_def f f') l = map (map_def g g') l.
 Proof.
-  intros.
-  eapply All_map_eq; red in X. apply forallb_All in H.
-  eapply All_impl. eapply All_prod. exact X. exact H.
-  intros [] [[] ?]; unfold map_def, test_def in *; cbn in *. rtoProp.
-  f_equal; eauto.
+  intros; eapply (@tfix_gen_forallb_map_spec A B (fun _ => True) P P' (fun _ => true)); eauto.
 Qed.
 
 Ltac apply_spec :=
@@ -371,6 +383,10 @@ Ltac apply_spec :=
     eapply (case_brs_forallb_map_spec H H')
   | H : tCaseBrsProp _ _ |- map _ _ = map _ _ =>
     eapply (case_brs_map_spec H)
+  | H : tFixProp_gen _ _ _ _, H' : forallb _ _ = _ |- map _ _ = map _ _ =>
+    eapply (tfix_gen_forallb_map_spec H H')
+  | H : tFixProp_gen _ _ _ _ |- map _ _ = map _ _ =>
+    eapply (tfix_gen_map_spec H)
   | H : tFixProp _ _ _, H' : forallb _ _ = _ |- map _ _ = map _ _ =>
     eapply (tfix_forallb_map_spec H H')
   | H : tFixProp _ _ _ |- map _ _ = map _ _ =>
@@ -574,12 +590,14 @@ Fixpoint noccur_between k n (t : term) : bool :=
   | tConst c u' => tConst c (subst_instance_instance u u')
   | tInd i u' => tInd i (subst_instance_instance u u')
   | tConstruct ind k u' => tConstruct ind k (subst_instance_instance u u')
-  | tLambda na T M => tLambda na (subst_instance_constr u T) (subst_instance_constr u M)
+  | tLambda na T M =>
+      tLambda (subst_instance_aname u na) (subst_instance_constr u T) (subst_instance_constr u M)
   | tApp f v => tApp (subst_instance_constr u f) (List.map (subst_instance_constr u) v)
-  | tProd na A B => tProd na (subst_instance_constr u A) (subst_instance_constr u B)
+  | tProd na A B =>
+      tProd (subst_instance_aname u na) (subst_instance_constr u A) (subst_instance_constr u B)
   | tCast c kind ty => tCast (subst_instance_constr u c) kind (subst_instance_constr u ty)
-  | tLetIn na b ty b' => tLetIn na (subst_instance_constr u b) (subst_instance_constr u ty)
-                                (subst_instance_constr u b')
+  | tLetIn na b ty b' => tLetIn (subst_instance_aname u na) (subst_instance_constr u b)
+                          (subst_instance_constr u ty) (subst_instance_constr u b')
   | tCase ind p c brs =>
     let p' := map_predicate (subst_instance_instance u) (subst_instance_constr u) (subst_instance_constr u) p in
     let brs' := List.map (map_branch (subst_instance_constr u)) brs in
@@ -622,16 +640,16 @@ Fixpoint closedu (k : nat) (t : term) : bool :=
 
 Fixpoint closedq (k : nat) (t : term) : bool :=
   match t with
-  | tSort univ => true
+  | tSort univ => closedq_sort k univ
   | tInd _ u => closed_instance_qualities k u
   | tConstruct _ _ u => closed_instance_qualities k u
   | tConst _ u => closed_instance_qualities k u
   | tRel i => true
   | tEvar ev args => forallb (closedq k) args
-  | tLambda _ T M | tProd _ T M => closedq k T && closedq k M
+  | tLambda na T M | tProd na T M => closedq_aname k na && closedq k T && closedq k M
   | tApp u v => closedq k u && forallb (closedq k) v
   | tCast c kind t => closedq k c && closedq k t
-  | tLetIn na b t b' => closedq k b && closedq k t && closedq k b'
+  | tLetIn na b t b' => closedq_aname k na && closedq k b && closedq k t && closedq k b'
   | tCase ind p c brs =>
     let p' := test_predicate (closed_instance_qualities k) (closedq k) (closedq k) p in
     let brs' := forallb (test_branch (closedq k)) brs in
