common/theories/Environment.v
@@ -192,7 +192,8 @@ Module Environment (T : Term).
     subst_context s k Γ =
     mapi (fun k' d => subst_decl s (Nat.pred #|Γ| - k' + k) d) Γ.
   Proof.
-    unfold subst_context, fold_context_k. rewrite rev_mapi. rewrite List.rev_involutive.
+    unfold subst_context, fold_context_k, fold_context_gen_k.
+    rewrite rev_mapi List.rev_involutive.
     apply mapi_ext. intros. f_equal. now rewrite List.length_rev.
   Qed.
 
@@ -204,11 +205,17 @@ Module Environment (T : Term).
   Definition subst_telescope s k (Γ : context) : context :=
     mapi (fun k' decl => map_decl (subst s (k' + k)) decl) Γ.
 
-  Global Instance subst_instance_decl : UnivSubst context_decl
-    := map_decl ∘ subst_instance.
+  #[global] Instance subst_instance_opt {A : Type} `{UnivSubst A} : UnivSubst (option A)
+    := fun u t => match t with
+               | Some t => Some (subst_instance u t)
+               | None => None
+               end.
+
+  #[global] Instance subst_instance_decl : UnivSubst context_decl
+    := fun u => map_decl_gen (subst_instance u) (subst_instance u).
 
   Global Instance subst_instance_context : UnivSubst context
-    := map_context ∘ subst_instance.
+    := fun u => map_context_gen (subst_instance u) (subst_instance u).
 
   Lemma subst_instance_length u (ctx : context)
     : #|subst_instance u ctx| = #|ctx|.
@@ -1199,7 +1206,10 @@ Module Environment (T : Term).
   Lemma context_assumptions_subst_instance u Γ :
     context_assumptions (subst_instance u Γ) =
     context_assumptions Γ.
-  Proof. apply context_assumptions_map. Qed.
+  Proof.
+    induction Γ; auto; cbn.
+    destruct (decl_body a); cbn; auto.
+  Qed.
 
   Lemma context_assumptions_subst_context s k Γ :
     context_assumptions (subst_context s k Γ) =
