template-rocq/theories/LiftSubst.v
@@ -456,7 +456,7 @@ Lemma map_vass_map_def g l n k :
   (mapi (fun i d => map_decl (lift n (i + k)) d) (mapi (fun i (d : def term) => vass (dname d) (lift0 i (dtype d))) l)).
 Proof.
   rewrite mapi_mapi mapi_map. apply mapi_ext.
-  intros. unfold map_decl, vass; simpl; f_equal.
+  intros. unfold map_decl, vass; simpl; cbv[map_decl_gen]; f_equal.
   rewrite permute_lift. lia. f_equal; lia.
 Qed.
 (*
